refactor(Normal Modal): consequence and remove nonempty

Logic/Modal/Normal/ModalCube.lean
@@ -11,36 +11,38 @@ import Logic.Modal.Normal.Completeness
 
 namespace LO.Modal.Normal
 
-def LogicalStrong (Λ₁ Λ₂ : AxiomSet β) := ∀ (p : Formula β), (⊧ᴹ[(𝔽(Λ₁) : FrameClass β)] p) → (⊧ᴹ[(𝔽(Λ₂) : FrameClass β)] p)
+def LogicalStrong {β} (Λ₁ Λ₂ : AxiomSet β) := ∀ {α}, ∀ (p : Formula β), (⊧ᴹ[(𝔽(Λ₁) : FrameClass α)] p) → (⊧ᴹ[(𝔽(Λ₂) : FrameClass α)] p)
 infix:20 " ≤ᴸ " => LogicalStrong
 
 namespace LogicalStrong
 
 instance : IsPreorder (AxiomSet β) (· ≤ᴸ ·) where
   refl := by simp_all [LogicalStrong];
-  trans := by intro Λ₁ Λ₂ Λ₃ h₁₂ h₂₃ p hF; exact h₂₃ p (h₁₂ p hF);
+  trans := by intro Λ₁ Λ₂ Λ₃ h₁₂ h₂₃ _ p hF; exact h₂₃ p (h₁₂ p hF);
 
 variable {α β : Type u}
 variable {Λ₁ Λ₂ : AxiomSet β}
 variable [Inhabited α] [DecidableEq β]
 
-lemma iff : (Λ₁ ≤ᴸ Λ₂) ↔ (∀ {F : Frame β}, (F ∈ 𝔽(Λ₂) → F ∈ (𝔽(Λ₁)))) := by
+lemma iff : (Λ₁ ≤ᴸ Λ₂) ↔ (∀ {α}, ∀ {F : Frame α}, (F ∈ 𝔽(Λ₂) → F ∈ (𝔽(Λ₁)))) := by
   constructor;
-  . intro h F hF₂ p hp;
+  . intro h _ F hF₂ p hp;
     exact h p (by simp [Formula.FrameClasses]; aesop) F hF₂;
-  . intro h₁ p h₂ F hF₂;
+  . intro h₁ _ p h₂ F hF₂;
+    have : F ∈ 𝔽(Λ₁) := h₁ hF₂;
     exact h₂ F $ h₁ hF₂;
 
-lemma not_iff : ¬(Λ₁ ≤ᴸ Λ₂) ↔ (∃ F ∈ 𝔽(Λ₂), (F : Frame β) ∉ 𝔽(Λ₁)) := by simpa using iff.not
+lemma not_iff : ¬(Λ₁ ≤ᴸ Λ₂) ↔ (∃ α, ∃ F ∈ 𝔽(Λ₂), (F : Frame α) ∉ 𝔽(Λ₁)) := by simpa using iff.not
 
-variable (hS : Λ₁ ≤ᴸ Λ₂)
+variable (hS : Λ₁ ≤ᴸ Λ₂) {Γ : Theory β} {p : Formula β}
 
-lemma consequence {Γ} {p : Formula β} : (Γ ⊨ᴹ[(𝔽(Λ₂) : FrameClass α)] p) → (Γ ⊨ᴹ[(𝔽(Λ₁) : FrameClass α)] p) := by
-  have := hS;
-  sorry;
+lemma consequence : (Γ ⊨ᴹ[(𝔽(Λ₁) : FrameClass α)] p) → (Γ ⊨ᴹ[(𝔽(Λ₂) : FrameClass α)] p) := by
+  intro h F hF₁;
+  exact h F $ iff.mp hS hF₁;
 
-lemma deducible (hComp : Completeness Λ₁ (𝔽(Λ₁) : FrameClass α)) {Γ} {p : Formula β} (hd : Γ ⊢ᴹ[Λ₂]! p) : Γ ⊢ᴹ[Λ₁]! p := by
-  exact hComp Γ p $ consequence hS $ AxiomSet.ssounds hd;
+lemma deducible (hComp : Completeness Λ₂ (𝔽(Λ₂) : FrameClass α)) (hd : Γ ⊢ᴹ[Λ₁]! p) : Γ ⊢ᴹ[Λ₂]! p := by
+  apply hComp;
+  exact consequence hS $ AxiomSet.ssounds hd;
 
 end LogicalStrong
 
@@ -52,11 +54,13 @@ namespace LogicStrictStronger
 instance : IsStrictOrder (AxiomSet β) (· <ᴸ ·) where
   irrefl := by simp [LogicalStrong]
   trans := by
-    simp [LogicalStrictStrong, LogicalStrong];
-    intro Λ₁ Λ₂ Λ₃ h₁₂ _ _ _ h₂₃ y _ _;
+    simp [LogicalStrong];
+    intro Λ₁ Λ₂ Λ₃ h₁₂ _ _ _ _ h₂₃ α₂ y _ _;
     constructor;
-    . intro p h₁; exact h₂₃ p $ h₁₂ p h₁;
-    . existsi y;
+    . intro _ p h₁;
+      exact h₂₃ p $ h₁₂ p h₁;
+    . simp [LogicalStrong];
+      existsi α₂, y;
       constructor;
       . simpa;
       . by_contra hn₁;
@@ -76,15 +80,11 @@ namespace LogicalEquivalence
 instance : IsEquiv (AxiomSet β) (· =ᴸ ·) where
   refl := by simp; apply IsRefl.refl;
   trans := by
-    simp;
-    intros _ _ _ h₁₂ h₂₁ h₂₃ h₃₂;
-    constructor;
-    . exact IsTrans.trans _ _ _ h₁₂ h₂₃;
-    . exact IsTrans.trans _ _ _ h₃₂ h₂₁;
+    simp; intros;
+    constructor <;> simp_all [LogicalStrong];
   symm := by
-    simp;
-    intros;
-    constructor <;> simpa;
+    simp; intros;
+    constructor <;> simp_all;
 
 variable {α₁ α₂ β} [Inhabited α₁] [Inhabited α₂] [DecidableEq β]
 
@@ -94,8 +94,8 @@ lemma deducible
   (hComp₂ : Completeness Λ₂ (𝔽(Λ₂) : FrameClass α₂))
   {Γ} {p : Formula β} : (Γ ⊢ᴹ[Λ₁]! p) ↔ (Γ ⊢ᴹ[Λ₂]! p) := by
   constructor;
-  . exact LogicalStrong.deducible h.2 hComp₂;
-  . exact LogicalStrong.deducible h.1 hComp₁;
+  . apply LogicalStrong.deducible h.1 hComp₂
+  . apply LogicalStrong.deducible h.2 hComp₁
 
 end LogicalEquivalence
 
@@ -122,12 +122,12 @@ end LogicKT
 theorem sstrong_KD_KT : (𝐊𝐃 : AxiomSet (Fin 2)) <ᴸ 𝐊𝐓 := by
   constructor;
   . apply LogicalStrong.iff.mpr;
-    intro F hF;
+    intro _ F hF;
     obtain hRefl := LogicKT.FrameClassDefinability.mpr hF;
     apply LogicKD.FrameClassDefinability.mp;
     exact serial_of_refl hRefl;
   . apply LogicalStrong.not_iff.mpr;
-    existsi (λ _ w₂ => w₂ = 1);
+    existsi _, (λ _ w₂ => w₂ = 1);
     constructor;
     . apply LogicKD.FrameClassDefinability.mp;
       simp [Serial];
@@ -139,14 +139,14 @@ theorem sstrong_KD_KT : (𝐊𝐃 : AxiomSet (Fin 2)) <ᴸ 𝐊𝐓 := by
 theorem sstrong_S4_S5 : (𝐒𝟒 : AxiomSet (Fin 3)) <ᴸ 𝐒𝟓 := by
   constructor;
   . apply LogicalStrong.iff.mpr;
-    intro F hF;
+    intro _ F hF;
     obtain ⟨hRefl, hEucl⟩ := LogicS5.FrameClassDefinability.mpr hF;
     apply LogicS4.FrameClassDefinability.mp;
     constructor;
     . exact hRefl;
     . exact trans_of_refl_eucl hRefl hEucl;
   . apply LogicalStrong.not_iff.mpr;
-    existsi (λ w₁ w₂ => (w₁ = w₂) ∨ (w₁ = 0 ∧ w₂ = 1) ∨ (w₁ = 0 ∧ w₂ = 2));
+    existsi (Fin 3), (λ w₁ w₂ => (w₁ = w₂) ∨ (w₁ = 0 ∧ w₂ = 1) ∨ (w₁ = 0 ∧ w₂ = 2));
     constructor;
     . apply LogicS4.FrameClassDefinability.mp;
       simp [Reflexive, Transitive];
@@ -192,12 +192,12 @@ end LogicKT4B
 theorem equivalent_S5_KT4B : (𝐒𝟓 : AxiomSet β) =ᴸ 𝐊𝐓𝟒𝐁 := by
   constructor;
   . apply LogicalStrong.iff.mpr;
-    intro F hF;
+    intro _ F hF;
     obtain ⟨hRefl, hTrans, hSymm⟩ := LogicKT4B.FrameClassDefinability.mpr hF;
     apply LogicS5.FrameClassDefinability.mp;
     exact ⟨hRefl, eucl_of_symm_trans hSymm hTrans⟩
   . apply LogicalStrong.iff.mpr;
-    intro F hF;
+    intro _ F hF;
     obtain ⟨hRefl, hEucl⟩ := LogicS5.FrameClassDefinability.mpr hF;
     apply LogicKT4B.FrameClassDefinability.mp;
     exact ⟨hRefl, trans_of_refl_eucl hRefl hEucl, symm_of_refl_eucl hRefl hEucl⟩
